\begin{answer}\\
Linear regression with regularization can be expressed in matrix form as \\
$(X\theta-y)^T (X\theta-y)+\lambda \theta^T \theta$\\
Note that in the class notes there was a $\frac{1}{2}$ term that neutralized the 2 coming out of the derivative, but it cancels out when we equate the derivative to zero so we can ignore it\\
$\therefore J(\theta)=(X\theta-y)^T (X\theta-y)+\lambda \theta^T \theta=(\theta^TX^TX \theta-\theta^TX^Ty -y^TX\theta+y^Ty) + \lambda \theta^T \theta$\\
$\therefore J(\theta)=tr \left [(X\theta-y)^T (X\theta-y)+\lambda \theta^T \theta=(\theta^TX^TX \theta-\theta^TX^Ty -y^TX\theta+y^Ty) + \lambda \theta^T \theta \right ]=tr(\theta^TX^TX \theta-\theta^TX^Ty -y^TX\theta+y^Ty) + tr(\lambda \theta^T \theta)$\\
$=tr(\theta^TX^TX \theta-\theta^TX^Ty -y^TX\theta+y^Ty) + \lambda tr(\theta^T \theta)$\\
Then $\nabla_{\theta}J(\theta)=\nabla_{\theta}tr(\theta^TX^TX \theta-\theta^TX^Ty -y^TX\theta+y^Ty)+\lambda \nabla_{\theta} tr(\theta^T \theta)$\\
In the class notes (lecture notes 1, page 11) we already derived $\nabla_{\theta}tr(\theta^TX^TX \theta-\theta^TX^Ty -y^TX\theta+y^Ty) = 2(X^TX\theta - X^Ty)$\\
We also know that $\nabla_{A} tr(ABA^TC)=CAB+C^TAB^T$. Let $A=\theta, B=I$ and $C=I$\\
Then $\nabla_{\theta}tr(\theta I \theta^T I)=I \theta I+ I \theta I = 2 \theta$\\
$\therefore \nabla_{\theta}J(\theta)=2(X^TX\theta - X^Ty - \lambda \theta)=2(X^TX\theta - X^Ty - \lambda I \theta)$\\
Setting this to zero we have
$2(X^TX\theta - X^Ty - \lambda I \theta)=0$\\
$\implies X^TX\theta  - \lambda I \theta= X^Ty$\\
$\implies (X^TX-\lambda I) \theta=X^Ty$\\
$\implies \theta=(X^TX-\lambda I)^{-1}X^Ty$\\
\end{answer}
