\begin{answer}\\
The covariance matrix is given by\\
$\sum=E[(X-E[X])(X-E[X])^T$\\
But we proved in the prev section that the expected value is zero\\
$\therefore Cov_{y \sim p(y;\theta)} \left[ \nabla_{\theta'}log p(y;\theta')|_{\theta'=\theta} \right] =E_{y \sim p(y;\theta)}[(\nabla_{\theta'}log p(y;\theta')-0)(\nabla_{\theta'}log p(y;\theta')-0)^T|_{\theta'=\theta}]$\\
$=E_{y \sim p(y;\theta)}[\nabla_{\theta'}log p(y;\theta') \nabla_{\theta'}log p(y;\theta')^T|_{\theta'=\theta}]$\\
\end{answer}
