\begin{answer}\\
We know that $(\frac{f}{g})'=\frac{f'g-g'f}{g^2}$\\
$\therefore (\frac{\nabla_{\theta'} p(y;\theta')}{p(y;\theta')})'=\frac{\nabla_{\theta'}^2 p(y;\theta')-\nabla_{\theta'}p(y;\theta')\nabla_{\theta'}p(y;\theta')^T}{p(y;\theta')p(y;\theta')}$\\
$=\frac{\nabla_{\theta'}^2 p(y;\theta')}{p(y;\theta')p(y;\theta')}-\frac{\nabla_{\theta'}p(y;\theta')\nabla_{\theta'}p(y;\theta')^T}{p(y;\theta')p(y;\theta')}=\frac{\nabla_{\theta'}^2 }{p(y;\theta')}-\frac{\nabla_{\theta'}p(y;\theta')}{p(y;\theta')} \left ( \frac{\nabla_{\theta'}p(y;\theta')}{p(y;\theta')} \right ) ^T$\\
$E_{y \sim p(y;\theta)} \left [ \nabla_{\theta'}^2 log p(y;\theta')|_{\theta'=\theta} \right]=E_{y \sim p(y;\theta)} \left [ \frac{\nabla_{\theta'}^2 }{p(y;\theta')}-\frac{\nabla_{\theta'}p(y;\theta')}{p(y;\theta')} \left ( \frac{\nabla_{\theta'}p(y;\theta')}{p(y;\theta')} \right ) ^T \right]$\\
$=E_{y \sim p(y;\theta)} \left [ \frac{\nabla_{\theta'}^2 }{p(y;\theta')} \right ] - E_{y \sim p(y;\theta)} \left [ \nabla_{\theta'} log p(y;\theta') \nabla_{\theta'} log p(y;\theta')^T \right ]$\\
$=\int_{-\infty}^{\infty}p(y;\theta') \frac{\nabla_{\theta'}^2 }{p(y;\theta')} dy - E_{y \sim p(y;\theta)} \left [ \nabla_{\theta'} log p(y;\theta') \nabla_{\theta'} log p(y;\theta')^T \right ]$\\
$=0-E_{y \sim p(y;\theta)} \left [ \nabla_{\theta'} log p(y;\theta') \nabla_{\theta'} log p(y;\theta')^T \right ] = -I(\theta)$\\
$\therefore I(\theta)=-E_{y \sim p(y;\theta)} \left [ \nabla_{\theta'}^2 log p(y;\theta')|_{\theta'=\theta} \right]=E_{y \sim p(y;\theta)} \left [ -\nabla_{\theta'}^2 log p(y;\theta')|_{\theta'=\theta} \right]$\\
\end{answer}
