\begin{answer}\\
$p(y;\eta)=b(y)e^{\eta y -a(\eta)}$\\
Since this is the probability density function, $\int_{- \infty}^{\infty}p(y;\eta)dy=1$\\
$\therefore \int_{- \infty}^{\infty}p(y;\eta)dy=\int b(y)e^{\eta y -a(\eta)}dy=1$\\
$\implies \int b(y)e^{\eta y} e^{-a(\eta)}dy=1$\\
$\implies e^{-a(\eta)} \int b(y)e^{\eta y}dy=1$\\
$\implies \int b(y)e^{\eta y}dy=e^{a(\eta)}$\\
$\implies log \int b(y)e^{\eta y}dy=a(\eta)$\\\\
$\therefore \frac{\partial a(\eta)}{\partial \eta}=\frac{\partial}{\partial \eta} log \int b(y)e^{\eta y}dy$\\
$=\frac{1}{\int b(y)e^{\eta y}dy} \frac{\partial}{\partial \eta} \int b(y)e^{\eta y}dy$\\
$=\frac{1}{e^{a(\eta)}} \int (\frac{\partial}{\partial \eta} b(y)e^{\eta y})dy$\\
$=\frac{1}{e^{a(\eta)}} \int y b(y)e^{\eta y}dy$\\
$\int y b(y)e^{\eta y - a(\eta)}dy=\int y p(y;\eta) = E[y|X; \theta]$\\
\end{answer}
