\begin{answer}\\
$\sum_{i=1}^{n}\sum_{j=i}^{n}z_ix_ix_jz_j=x_i^2+2x_1z_1x_2z_2+\dots+2x_1z_1x_nz_n+x_2^2z_2^2+2x_2z_2x_3z_3+\dots+x_n^2z_n^2$\\
$(x^Tz)^2=x_i^2+2x_1z_1x_2z_2+\dots+2x_1z_1x_nz_n+x_2^2z_2^2+2x_2z_2x_3z_3+\dots+x_n^2z_n^2$\\
$\therefore \sum_{i=1}^{n}\sum_{j=i}^{n}z_ix_ix_jz_j=(x^Tz)^2 \geq 0$\\
$J(\theta)=-\frac{1}{m}\sum_{i=1}^{m}\left[ y^{(i)}log(g(\theta^T z^{(i)})) + (1-y^{(i)})log(1-g(\theta^T z^{(i)})) \right]$\\
$=\frac{1}{m}\sum_{i=1}^{m} - \left[ y^{(i)}log(g(\theta^T x^{(i)})) + (1-y^{(i)})log(1-g(\theta^T x^{(i)})) \right]$\\
We can ignore the $\frac{1}{m}$ in the derivative since it is a constant and doesnt change the calculations\\
$\therefore \frac{\partial J}{\partial \theta_j}=-(y \frac{1}{g(\theta^T x)}g(\theta^T x)(1-g(\theta^T x))x_j + (1-y)\frac{1}{1-g(\theta^T x)}-g(\theta^T x)(1-g(\theta^T x))x_j)$
$=-(yx_j-yx_jg(\theta^T x)-g(\theta^T x)x_j +yx_jg(\theta^T x))= g(\theta^T x)x_j -yx_j$\\

$\therefore \frac{\partial J^2}{\partial \theta_1^2}=g(\theta^T x)(1-g(\theta^T x))x_1^2$, $\frac{\partial J^2}{\partial \theta_1\theta_2}=g(\theta^T x)(1-g(\theta^T x))x_1x_2$ and so on...\\
$\therefore H=$
\[
\begin{bmatrix}
g(\theta^T x)(1-g(\theta^T x))x_1^2 & g(\theta^T x)(1-g(\theta^T x))x_1x_2 & \dots & g(\theta^T x)(1-g(\theta^T x))x_1x_n \\
g(\theta^T x)(1-g(\theta^T x))x_1x_2 & g(\theta^T x)(1-g(\theta^T x))x_2^2 & \dots & g(\theta^T x)(1-g(\theta^T x))x_2x_n \\
\vdots & \vdots & \vdots  & \vdots \\
g(\theta^T x)(1-g(\theta^T x))x_1x_n & g(\theta^T x)(1-g(\theta^T x))z_2x_n & \dots & g(\theta^T x)(1-g(\theta^T x))x_n^2 \\
\end{bmatrix}
\]=$g(\theta^T x)(1-g(\theta^T x))$
\[
\begin{bmatrix}
x_1^2 & x_1x_2 & \dots & x_1x_n \\
x_1x_2 & x_2^2 & \dots & x_2x_n \\
\vdots & \vdots & \vdots  & \vdots \\
x_1x_n & z_2x_n & \dots & x_n^2 \\
\end{bmatrix}
\]\\
but $0 \leq g(\theta^T x) \leq 1$ since its the sigmoid function. Also $0 \leq (1-g(\theta^T x)) \leq1$\\
$\therefore z^THz=g(\theta^T x)(1-g(\theta^T x))(z_1^2x_1^2+2z_1x_1x_2z_2+\dots+z_n^2x_n^2)=g(\theta^T x)(1-g(\theta^T x))(x^Tz)^2$\\
we already showed $(x^Tz)^2 \geq 0$\\
$\therefore z^THz \geq 0$
\end{answer}