\begin{answer}\\
$p(y=1|x;\phi,\mu_0,\mu_1,\sigma)=\frac{p(x|y=1;\phi,\mu_0,\mu_1,\sigma)p(y=1;\phi,\mu_0,\mu_1,\sigma)}{p(x;\phi,\mu_0,\mu_1,\sigma)}$\\
$=\frac{p(x|y=1;\phi,\mu_0,\mu_1,\sigma)p(y=1;\phi,\mu_0,\mu_1,\sigma)}{p(x|y=1;\phi,\mu_0,\mu_1,\sigma)p(y=1)+p(x|y=0;\phi,\mu_0,\mu_1,\sigma)*p(y=0)}$\\
$=\frac{\frac{1}{(2 \pi)^{n/2}| \sum | ^{1/2}} exp(-\frac{1}{2}(x-\mu_1)^T\sum^{-1}(x-\mu_1))\phi}{\frac{1}{(2 \pi)^{n/2}| \sum | ^{1/2}} exp(-\frac{1}{2}(x-\mu_1)^T\sum^{-1}(x-\mu_1))\phi+\frac{1}{(2 \pi)^{n/2}| \sum | ^{1/2}} exp(-\frac{1}{2}(x-\mu_0)^T\sum^{-1}(x-\mu_0))(1-\phi)}$\\
$=\frac{1}{1+\frac{1-\phi}{phi}exp(-\frac{1}{2}(x-\mu_0)^T\sum^{-1}(x-\mu_0)+\frac{1}{2}(x-\mu_1)^T\sum^{-1}(x-\mu_1))}$\\
$=\frac{1}{1+exp(log(\frac{1-\phi}{phi})-\frac{1}{2}((x-\mu_0)^T\sum^{-1}(x-\mu_0)-(x-\mu_1)^T\sum^{-1}(x-\mu_1)))}$\\
lets expand the term\\
$(x-\mu_0)^T\sum^{-1}(x-\mu_0)-(x-\mu_1)^T\sum^{-1}(x-\mu_1)$\\
$=x^T\sum^{-1}x-x^T\sum^{-1}\mu_0-\mu_0^T\sum^{-1}x+\mu_0^T\sum^{-1}\mu_0-x^T\sum^{-1}x+x^T\sum^{-1}\mu_1+\mu_1^T\sum^{-1}x-\mu_1^T\sum^{-1}\mu_1$\\
$=-x^T\sum^{-1}\mu_0-\mu_0^T\sum^{-1}x+\mu_0^T\sum^{-1}\mu_0+x^T\sum^{-1}\mu_1+\mu_1^T\sum^{-1}x-\mu_1^T\sum^{-1}\mu_1$\\
$=-\mu_0^T\sum^{-1}x-\mu_0^T\sum^{-1}x+\mu_0^T\sum^{-1}\mu_0+\mu_1^T\sum^{-1}x+\mu_1^T\sum^{-1}x-\mu_1^T\sum^{-1}\mu_1$\\
$=-2\mu_0^T\sum^{-1}x+\mu_0^T\sum^{-1}\mu_0+2\mu_0^T\sum^{-1}x-\mu_1^T\sum^{-1}\mu_1$\\
$=2(\mu_1-\mu_0)^T\sum^{-1}x+\mu_0^T\sum^{-1}\mu_0-\mu_1^T\sum^{-1}\mu_1$\\
$\therefore p(y=1|x;\phi,\mu_0,\mu_1,\sigma)=\frac{1}{1+exp(log\frac{1-\phi}{\phi}+\frac{1}{2}(\mu_0^T\sum^{-1}\mu_0-\mu_1^T\sum^{-1}\mu_1)+(\mu_1-\mu_0)^T\sum^{-1}x)}$\\
let $\theta=(\mu_1-\mu_0)^T\sum^{-1}=\sum^{-1}(\mu_1-\mu_0)$ and\\
$\theta_0=\frac{1}{2}(\mu_0^T\sum^{-1}\mu_0-\mu_1^T\sum^{-1}\mu_1)-log(\frac{1-\phi}{\phi})$\\
then $p(y=1|x;\phi,\mu_0,\mu_1,\sigma)=\frac{1}{1+exp(-(\theta^Tx+\theta_0))}$\\
\end{answer}
