\begin{answer}\\
We know that the exponential family is given by $p(y;\lambda)=b(y)e^{\eta^T T(y)-a(\eta)}$\\
So, on our case let us factor the equation into that format\\
$p(y;\lambda)=\frac{e^{-\lambda}\lambda^y}{y!}=\frac{1}{y!}e^{-\lambda}\lambda^y=\frac{1}{y!}e^{-\lambda}e^{y log \lambda}=\frac{1}{y!}e^{y log \lambda-\lambda}$\\
Therefore we have\\
$b(y)=\frac{1}{y!}$\\
$\eta=log \lambda$\\
$T(y)=y$\\
$a(\eta)=\lambda=e^{\eta}$\\
\\
$\therefore p(y;\eta)=\frac{1}{y!}e^{\eta y -e^{\eta}}$\\
\end{answer}
