\begin{answer}\\
We add the bias term $x_0=1$ and $h_0=1$\\
Let\\
$z_1^{[2]}=w_{01}^{[1]}x_0+w_{11}^{[1]}x_1+w_{21}^{[1]}x_2$ and $h_1=\sigma(z_1^{[2]})$\\
$z_2^{[2]}=w_{02}^{[1]}x_0+w_{12}^{[1]}x_1+w_{22}^{[1]}x_2$ and $h_2=\sigma(z_2^{[2]})$\\
$z_3^{[2]}=w_{03}^{[1]}x_0+w_{13}^{[1]}x_1+w_{23}^{[1]}x_2$ and $h_2=\sigma(z_3^{[2]})$\\
\\
$z^{[3]}=w_0^{[2]}h_0+w_1^{[2]}h_1+w_2^{[2]}h_2+w_3^{[2]}h_3$\\
$o=\sigma(z^{[3]})$\\
$l=\frac{1}{m}\sum_{i=1}^{m}(o^{(i)}-y^{(i)})^2$\\
We can see that $w_{12}^{[1]}$ is only present in $z_2^{[2]}$ so when we do back prop we can ignore the other terms.\\
$\therefore \frac{\partial l}{\partial w_{12}^{[1]}}=\frac{\partial l}{\partial o}\frac{\partial o}{\partial z^{[3]}}\frac{\partial z^{[3]}}{\partial h_2}\frac{\partial h_2}{\partial z_2^{[2]}}\frac{\partial z_2^{[2]}}{\partial w_{12}^{[1]}}$\\
$=2(o-y)o(1-o)w_2^{[2]} \sigma(z_2^{[2]})(1-\sigma(z_2^{[2]}))x_1$\\
$=2(o-y)o(1-o)w_2^{[2]} \sigma(w_{02}^{[1]}x_0+w_{12}^{[1]}x_1+w_{22}^{[1]}x_2)(1-\sigma(w_{02}^{[1]}x_0+w_{12}^{[1]}x_1+w_{22}^{[1]}x_2))x_1$\\
\end{answer}