\begin{answer}\\
Since all labeled examples are positive\\
$p(y^{(i)}|x^{(i)})=p(t^{(i)}=1 \cap y^{(i)}=1|x)$\\
Using the chain rule we have\\
$p(y^{(i)}=1|x^{(i)})=p(t^{(i)}=1|x)p(y^{(i)}=1|t^{(i)}=1,x^{(i)})$\\\\
But since $y^{(i)}$ and $x^{(i)}$ are conditionally independant given $t^{(i)}$\\
$p(y^{(i)}=1|t^{(i)}=1,x^{(i)})=p(y^{(i)}=1|t^{(i)}=1)$\\\\
$\therefore p(y^{(i)}=1|x^{(i)})=p(t^{(i)}=1|x)p(y^{(i)}=1|t^{(i)}=1)$\\
$\implies p(t^{(i)}=1|x)=p(y^{(i)}=1|x) \frac{1}{p(y^{(i)}=1|t^{(i)}=1)}$\\
Let $\alpha=p(y^{(i)}=1|t^{(i)}=1)$ then $p(t^{(i)}=1|x)=p(y^{(i)}=1|x)/\alpha$
\end{answer}
